src/impl/TLS13.Impl.Server.fsti
@@ -161,6 +161,56 @@ fn process_select_server_parameters
                    network_out_bytes
                    app_out_bytes)
 
+fn process_send_server_hello
+  (s:server)
+  (raw:array U8.t)
+  (raw_len:SZ.t)
+  (fragment:array U8.t)
+  (fragment_len:SZ.t)
+  (lsh:IM.server_hello)
+  (#sh:erased M.server_hello)
+  (network_out:array U8.t)
+  (network_out_len:SZ.t)
+  (app_out:array U8.t)
+  (app_out_len:SZ.t)
+  requires connection_exactly s 'st0 **
+           pts_to raw 'raw_bytes **
+           pts_to fragment 'fragment_bytes **
+           IM.is_valid_server_hello lsh sh **
+           pts_to network_out 'old_network_out **
+           pts_to app_out 'old_app_out **
+           pure (B.length 'raw_bytes == SZ.v raw_len /\
+                 B.length 'fragment_bytes == SZ.v fragment_len /\
+                 B.length 'old_network_out == SZ.v network_out_len /\
+                 B.length 'old_app_out == SZ.v app_out_len /\
+                 SZ.v raw_len <= SZ.v network_out_len /\
+                 Seq.equal
+                    (Seq.slice (Ghost.reveal 'old_network_out) 0 (SZ.v raw_len))
+                    (Ghost.reveal 'raw_bytes) /\
+                 Seq.equal
+                    (Ghost.reveal 'fragment_bytes)
+                    (TLS13.Wire.Spec.serialize_handshake (M.ServerHello sh)) /\
+                 SZ.v fragment_len <= Bounds.max_server_hello_len /\
+                 ST.server_end_to_end_invariant 'st0 /\
+                 CM.can_send_server_hello 'st0 sh (Ghost.reveal 'raw_bytes))
+  returns resp:ST.server_response
+  ensures exists* st1 network_out_bytes app_out_bytes.
+          connection_exactly s st1 **
+          pts_to raw 'raw_bytes **
+          pts_to fragment 'fragment_bytes **
+          pts_to network_out network_out_bytes **
+          pts_to app_out app_out_bytes **
+          pure (B.length network_out_bytes == SZ.v network_out_len /\
+                B.length app_out_bytes == SZ.v app_out_len /\
+                ST.server_local_event_end_to_end_correct
+                   'st0
+                   st1
+                   resp
+                   ST.LocalSendServerHello
+                   B.empty
+                   network_out_bytes
+                   app_out_bytes)
+
 fn process_client_hello
   (s:server)
   (raw:array U8.t)
